**T2**
$$
L_2(x) = \frac{(x-1)(x-2)}{(-1-1)(-1-2)}\cdot f(-1)+\frac{(x+1)(x-2)}{(1+1)(1-2)}\cdot f(1)+\frac{(x+1)(x-1)}{(2+1)(2-1)}\cdot f(2)  \\
= -\frac{1}{2}(x-1)(x-2) + \frac{4}{3}(x+1)(x-1)  \\
= \frac{5}{6}x^2 + \frac{3}{2}x - \frac{7}{3}
$$


**T3**

* 线性
  $$
  f(x) = f(x_0)+f[x_0,x_1](x-x_0)  \\
  = f(x_0) + \frac{f(x_1)-f(x_0)}{x_1 - x_0}\cdot (x-x_0)  \\
  = -0.693147 + \frac{-0.510826+0.693147}{0.1}\cdot(0.54-0.5)  \\
  = -0.620219
  $$
  
* 二次
  $$
  f(x) = f(x_0) + f[x_0,x_1](x-x_0) + f[x_0,x_1,x_2](x-x_0)(x-x_1) \\
  = f(x_0) + f[x_0,x_1](x-x_0) + \frac{f[x_1,x_2]-f[x_0,x_1]}{x_2-x_0}\cdot (x-x_0)(x-x_1)  \\
  = -0.616107
  $$
  

**T4**
$$
f(x) = f(x_0)+f[x_0,x_1](x-x_0)+R_1(x)  \\
r = 0.5 * 10^{-5} + 0.5 * 10^{-5} + \frac{f''(\xi)}{2}(\frac{\pi}{2*10800})^2 \\
  = 0.1*10^{-4} + 1.06*10^{-8}
$$



**T6**

(1) let $y=f(x)=x^k$

$f(x) =  \sum_{j=0}^n x_j^k l_j(x) + R(x)$ , however the power is less than k, the Lagrange function should be determined as the only one. for i in range(0,n) $f(x_i) =  \sum_{j=0}^n x_j^k l_j(x_i)$ , which means $f(x)=x^k$ is one solotion. so that $R(x)=0$. $\sum_{j=0}^n x_j^k l_j(x)=x^k$

(2)the left side could be expanded
$$
\sum_{j=0}^n (x_j-x)^kl_j(x)=\sum_{j=0}^nl_j(x)\sum_{i=0}^k C_k^ix_j^{k-i}(-x)^i  \\
= \sum_{i=0}^kC_k^i(-x)^{i}\cdot\sum_{j=0}^n x_j^{k-i} l_j(x)  \\
= \sum_{i=0}^kC_k^i(-x)^{i}\cdot x^{k-i} \ (from (1))  \\
=(x-x)^k = 0
$$


**T8**
$$
R_2(x) = \frac{t(t-1)(t-2)}{6}h^3f^{(3)}(\xi) \\
\leq \frac{2\sqrt{3}}{9}h^3\cdot e^4 \leq 10^{-6}  \\
h \leq 0.006
$$
**T19**
$$
H_3(x) = y_0\alpha_0(x)+y_1\alpha_1(x)+y'_0\beta_0(x)+y'_1\beta_1(x) \\
\alpha_0(x) = (1+2l_1(x))l_0^2(x) = (1+2x)(x-1)^2 \\
\alpha_1(x) = (1+2l_0(x))l_1^2(x) = (3-2x)x^2 \\
\beta_0(x) = (x-x_0)l_0^2(x) = x(x-1)^2 \\
\beta_1(x) = (x-x_1)l_1^2(x) = (x-1)x^2 \\
H_3(x) = \alpha_1(x)+\beta_1(x) = (2-x)x^2  \\
part\ one\ of\ P(x)\ is\ above\\
part\ 2\ H_4(x)\\
H_4(0)=H_4'(0)=H_4(1)=H_4'(1)=0  \\
let\ H_4(x)=ax^2(x-1)^2  \\
H_4(2) = 1 \rightarrow a=\frac{1}{4} \\
P(x) = (2-x)x^2+\frac{1}{4}x^2(x-1)^2 = \frac{1}{4}x^2(x-3)^2
$$
