**T2**

$y_{n+1} = y_n + \frac{h}{2}[f(x_n,y_n)+f(x_n+h, y_n+hf(x_n,y_n))]$

y(0)=1

y(0.1)=1+0.05*(1+0+0.1+1+0.1*(0+1))=1.11

y(0.2)=1.06+0.05(0.1+1.06+0.2+1.06+0.1*(0.1+1.06))=1.24205

y(0.3)=1.39846525

y(0.4)=1.5818041012500001

y(0.5)=1.7948935318812502



y(0.1)=1.1103418361512953
y(0.2)=1.2428055163203398
y(0.3)=1.3997176151520059
y(0.4)=1.5836493952825408
y(0.5)=1.7974425414002564



**T6**
$$
\left\{
	\begin{array}{cc}
		K1 =& f(x_n, y_n) \\
		K2 =& f(x_n + \frac{h}{2}, y_n + \frac{h}{2}K1) \\
		K3 =& f(x_n + \frac{h}{2}, y_n + \frac{h}{2}K2) \\
		K4 =& f(x_n + h, y_n + hK3) \\
		y_{n+1} =& y_n + \frac{h}{6}(K1 + 2K2 + 2K3 + K4) \\
	\end{array}
\right.
$$


y(0.2)=1.727548209366391
y(0.4)=2.7429512988953544
y(0.6)=4.094181355422614
y(0.8)=5.829210728361705
y(1.0)=7.996012143148541



**T9**

$y' = -2xe^{-x^2}$ 

$y'' = (4x^2-2)e^{-x^2}$

$y''' = (-8x^3+12x)e^{-x^2}$ 

二阶： $y(x+h) = y(x) + hy'(x) + \frac{1}{2}h^2y''(x)$ 

三阶： $y(x+h) = y(x) + hy'(x) + \frac{1}{2}h^2y''(x) + \frac{1}{6}h^3y'''(x)$ 



显式：$y_{n+1}=y_n+\frac{h}{2}(3f_n-f_{n-1}) = y_n + \frac{h}{2}(2-3y_n+y_{n-1})$  , $y(1.0)=0.626$

隐式： $y_{n+1} = y_n + \frac{h}{2}(f_{n}+f_{n+1}) = y_n + \frac{h}{2}(2-y_n-y_{n+1})$     , $y(1.0)=0.633$

$y(1.0)=0.6321$

 















